Examples/SignedDHKEM/DiffieHellman.lean
@@ -168,7 +168,7 @@ def dh.attackerKnowledge [BytesFunctor] [BytesFunctor.Has SubF]: SubAttackerKnow
   pred p out :=
     ∃ pk sk,
       out = dh pk sk ∧
-      Kleene.Forall p [pk, sk]
+      Fixpoint.Forall p [pk, sk]
 
 #combine [BytesFunctor.Has SubF] into attackerKnowledge' from
   dhPk,
@@ -198,7 +198,7 @@ theorem attacker_knows_dh
 := by
   intro h_pk h_sk
   apply Bytes.AttackerKnows.prove dh.attackerKnowledge
-  simp only [dh.attackerKnowledge, Kleene.Forall]
+  simp only [dh.attackerKnowledge, Fixpoint.Forall]
   grind
 
 end AttackerKnowledge
@@ -625,7 +625,7 @@ instance: SubAttackerKnowledgeTheorem dh.attackerKnowledge where
     simp only [dh.attackerKnowledge]
     intro out tr h_tr ⟨pk, sk, ⟨ h_out, h_inputs ⟩⟩
     subst h_out
-    simp_all [Bytes.Publishable, Kleene.Forall]
+    simp_all [Bytes.Publishable, Fixpoint.Forall]
     grind [dh.Invariant, canFlowTrans]
 
 end AttackerKnowledgeTheorem
